cedar-lean/Cedar/Thm/Validation/EnvironmentValidation.lean
@@ -1,0 +1,171 @@
+/-
+ Copyright Cedar Contributors
+
+ Licensed under the Apache License, Version 2.0 (the "License");
+ you may not use this file except in compliance with the License.
+ You may obtain a copy of the License at
+
+      https://www.apache.org/licenses/LICENSE-2.0
+
+ Unless required by applicable law or agreed to in writing, software
+ distributed under the License is distributed on an "AS IS" BASIS,
+ WITHOUT WARRANTIES OR CONDITIONS OF ANY KIND, either express or implied.
+ See the License for the specific language governing permissions and
+ limitations under the License.
+-/
+
+import Cedar.Validation.EnvironmentValidator
+import Cedar.Thm.Validation.Validator
+
+/-!
+This file proves that various `*.validateWellFormed` functions
+correctly implement their spec versions.
+-/
+
+namespace Cedar.Thm
+
+open Cedar.Data
+open Cedar.Spec
+open Cedar.Validation
+
+theorem entity_type_validate_well_formed_is_sound
+  {env : Environment} {ety : EntityType}
+  (hok : EntityType.validateWellFormed env ety = .ok ()) :
+  EntityType.WellFormed env ety
+:= by
+  simp only [
+    EntityType.validateWellFormed,
+    List.any_eq_true, beq_iff_eq, Prod.exists,
+    exists_and_right, ite_eq_left_iff, Bool.not_eq_true,
+    not_exists, not_and, forall_exists_index,
+    reduceCtorEq, imp_false, Classical.not_forall,
+    not_imp, Decidable.not_not,
+  ] at hok
+  simp only [EntityType.WellFormed, ActionSchema.IsActionEntityType]
+  cases h : env.ets.contains ety
+  · have ⟨uid, entry, hacts, heq⟩ := hok h
+    simp only [Bool.false_eq_true, false_or]
+    exists uid
+    simp only [heq, and_true]
+    simp only [Map.toList] at hacts
+    have : (List.find? (fun x => x.fst == uid) (Map.kvs env.acts)).isSome
+    := by
+      apply List.find?_isSome.mpr
+      exists (uid, entry)
+      simp [hacts]
+    cases h : List.find? (fun x => x.fst == uid) (Map.kvs env.acts)
+    · simp [h] at this
+    · simp [ActionSchema.contains, Map.find?, h]
+  · simp [h]
+
+mutual
+
+theorem validate_attrs_well_formed_is_sound
+  {env : Environment} {rty} {attr : Attr} {qty : QualifiedType}
+  (hwf : (Map.mk rty).WellFormed)
+  (hok : validateAttrsWellFormed env rty = .ok ())
+  (hfind : (Map.mk rty).find? attr = some qty) :
+  QualifiedType.WellFormed env qty
+:= by
+  cases rty with
+  | nil => simp [Map.find?, List.find?] at hfind
+  | cons hd tl =>
+    simp only [Map.toList, validateAttrsWellFormed] at hok
+    cases h : hd.snd with
+    | optional attr_ty =>
+      simp only [h, bind, Except.bind] at hok
+      split at hok
+      · contradiction
+      · rename_i hwf_hd
+        have := (Map.in_list_iff_find?_some hwf).mpr hfind
+        simp only [Map.kvs, List.mem_cons] at this
+        cases this with
+        | inl hhd =>
+          have e : qty = hd.snd := by simp [← hhd]
+          simp only [e, h]
+          constructor
+          exact type_validate_well_formed_is_sound hwf_hd
+        | inr htl =>
+          have hwf_tl : (Map.mk tl).WellFormed
+          := Map.wf_implies_tail_wf hwf
+          have := (Map.in_list_iff_find?_some hwf_tl).mp htl
+          exact validate_attrs_well_formed_is_sound hwf_tl hok this
+    | required attr_ty =>
+      simp only [h, bind, Except.bind] at hok
+      split at hok
+      · contradiction
+      · rename_i hwf_hd
+        have := (Map.in_list_iff_find?_some hwf).mpr hfind
+        simp only [Map.kvs, List.mem_cons] at this
+        cases this with
+        | inl hhd =>
+          have e : qty = hd.snd := by simp [← hhd]
+          simp only [e, h]
+          constructor
+          exact type_validate_well_formed_is_sound hwf_hd
+        | inr htl =>
+          have hwf_tl : (Map.mk tl).WellFormed
+          := Map.wf_implies_tail_wf hwf
+          have := (Map.in_list_iff_find?_some hwf_tl).mp htl
+          exact validate_attrs_well_formed_is_sound hwf_tl hok this
+termination_by sizeOf rty
+decreasing_by
+  any_goals
+    have h : rty = hd :: tl := by assumption
+    simp [h]
+    omega
+  -- optional attribute
+  any_goals
+    have h : rty = hd :: tl := by assumption
+    try have hsnd : hd.snd = Qualified.optional attr_ty := by assumption
+    try have hsnd : hd.snd = Qualified.required attr_ty := by assumption
+    calc
+      sizeOf attr_ty < sizeOf hd := by
+        simp [←hhd]
+        simp [e, hsnd]
+        omega
+      _ < sizeOf rty := by
+        simp [h]
+        omega
+
+theorem type_validate_well_formed_is_sound
+  {env : Environment} {ty : CedarType}
+  (hok : ty.validateWellFormed env = .ok ()) :
+  CedarType.WellFormed env ty
+:= by
+  cases ty with
+  | bool _ | int | string | ext _ => constructor
+  | entity ety =>
+    simp only [CedarType.validateWellFormed] at hok
+    constructor
+    exact entity_type_validate_well_formed_is_sound hok
+  | set ty =>
+    simp only [CedarType.validateWellFormed] at hok
+    constructor
+    exact type_validate_well_formed_is_sound hok
+  | record rty =>
+    -- Some simplifications
+    simp only [
+      CedarType.validateWellFormed,
+      Except.bind_ok,
+      Except.bind_err,
+    ] at hok
+    cases hwf_rty : rty.wellFormed
+    · simp only [hwf_rty, Bool.false_eq_true, ↓reduceIte, reduceCtorEq] at hok
+    simp only [hwf_rty, ↓reduceIte] at hok
+    replace hwf_rty := Map.wellFormed_correct.mp hwf_rty
+    constructor
+    · exact hwf_rty
+    -- Soundness of `CedarType.validateWellFormed.validateAttrsWellFormed`
+    · intros _ _ hfind
+      exact validate_attrs_well_formed_is_sound hwf_rty hok hfind
+termination_by sizeOf ty
+decreasing_by
+  any_goals simp [*]
+  · cases rty
+    simp
+    omega
+
+end
+
+end Cedar.Thm
